src/SimultSubst.v
@@ -1,0 +1,277 @@
+From Equations Require Import Equations.
+From stdpp Require Import base gmap.
+From MRC Require Import Prelude.
+From MRC Require Import Stdppp.
+From MRC Require Import SeqNotation.
+From MRC Require Import Model.
+From MRC Require Import PredCalcBasic.
+From MRC Require Import PredCalcEquiv.
+From MRC Require Import PredCalcSubst.
+From MRC Require Import PredCalcFacts.
+
+Section simult_subst.
+  Context {M : model}.
+
+  Local Notation term := (term (value M)).
+  Local Notation atomic_formula := (atomic_formula (value M)).
+  Local Notation formula := (formula (value M)).
+
+  Implicit Types x y : variable.
+  Implicit Types t : term.
+  Implicit Types af : atomic_formula.
+  Implicit Types A : formula.
+  Implicit Types m : gmap variable term.
+
+  Fixpoint simult_subst_term t m :=
+    match t with
+    | TConst v => TConst v
+    | TVar x =>
+        match m !! x with
+        | Some t' => t'
+        | None => TVar x
+        end
+    | TApp sym args => TApp sym (map (λ arg, simult_subst_term arg m) args)
+    end.
+
+  Definition simult_subst_af af m :=
+    match af with
+    | AT_Eq t₁ t₂ => AT_Eq (simult_subst_term t₁ m) (simult_subst_term t₂ m)
+    | AT_Pred sym args => AT_Pred sym (map (fun arg => simult_subst_term arg m) args)
+    | _ => af
+    end.
+
+  Definition simult_subst_map_fvars m : gset variable :=
+    ⋃ (term_fvars ∘ snd <$> map_to_list m).
+
+  Definition quant_simult_subst_fvars y A m :=
+    (formula_fvars A ∖ {[y]}) ∪ simult_subst_map_fvars m ∪ dom m.
+
+  Lemma quant_simult_subst_fvars_inv y' y A m :
+    y' ∉ quant_simult_subst_fvars y A m →
+    (y = y' ∨ y' ∉ formula_fvars A) ∧ (y' ∉ dom m) ∧ (∀ x t, m !! x = Some t → y' ∉ term_fvars t).
+  Proof with auto.
+    intros. unfold quant_simult_subst_fvars in H. do 2 rewrite not_elem_of_union in H.
+    destruct_and! H. split_and!...
+    - apply not_elem_of_difference in H. set_solver.
+    - clear H H1. unfold simult_subst_map_fvars in H2. unfold not in H2.
+      rewrite elem_of_union_list in H2. intros. destruct (decide (y' ∈ term_fvars t))...
+      exfalso. apply H2. clear H2. exists (term_fvars t). split...
+      assert (<[x:=t]> (delete x m) = m) as <- by (apply insert_delete; assumption).
+      rewrite map_to_list_insert.
+      2:{ rewrite lookup_delete... }
+      simpl. apply elem_of_cons. left...
+  Qed.
+
+  Equations? simult_subst A m : formula by wf (rank A) lt :=
+    simult_subst (FAtom af) m => FAtom (simult_subst_af af m);
+    simult_subst (FNot A) m => FNot (simult_subst A m);
+    simult_subst (FAnd A₁ A₂) m => FAnd
+                        (simult_subst A₁ m)
+                        (simult_subst A₂ m);
+    simult_subst (FOr A₁ A₂) m => FOr
+                       (simult_subst A₁ m)
+                       (simult_subst A₂ m);
+    simult_subst (FExists y A) m =>
+        let y' := fresh_var y (quant_simult_subst_fvars y A m) in
+        FExists y' (simult_subst (A[y \ y']) m).
+  Proof.
+    all: try (simpl; lia).
+    unfold rank. simpl. fold Nat.add. pose proof (subst_preserves_shape A y (y')).
+    deduce_rank_eq H. rewrite Hfr. rewrite Hqr. lia.
+  Qed.
+
+  Definition to_simult_subst_map (xs : list variable) (ts : list term)
+    `{LengthEqLists variable term xs ts}: gmap variable term := list_to_map (zip xs ts).
+
+
+  Notation "A [[ xs \ ts ]]" := (simult_subst A (to_simult_subst_map xs ts))
+                              (at level 10, left associativity,
+                                xs custom seq_notation,
+                                ts custom seq_notation) : refiney_scope.
+
+  Notation "A [[ xs \ ts ]]" := (simult_subst A (to_simult_subst_map xs ts))
+                              (in custom formula at level 74, left associativity,
+                                xs custom seq_notation,
+                                ts custom seq_notation) : refiney_scope.
+
+  Lemma simult_subst_term_id t m :
+    term_fvars t ∩ dom m = ∅ →
+    simult_subst_term t m = t.
+  Proof with auto.
+    intros H. induction t; simpl...
+    - simpl in H. replace (m !! x) with (@None term)... symmetry.
+      rewrite <- not_elem_of_dom. set_solver.
+    - f_equal. induction args... simpl. f_equal.
+      + apply H0; [left; auto | set_solver].
+      + apply IHargs; [naive_solver | set_solver].
+  Qed.
+
+  Lemma simult_subst_af_id af m :
+    af_fvars af ∩ dom m = ∅ →
+    simult_subst_af af m = af.
+  Proof with auto.
+    intros H.
+    destruct af...
+    - simpl. simpl in H. do 2 rewrite simult_subst_term_id by set_solver...
+    - simpl. f_equal. induction args... simpl in H. simpl in *. f_equal.
+      + rewrite simult_subst_term_id... set_solver.
+      + apply IHargs. set_solver.
+  Qed.
+
+  Tactic Notation "generalize_fresh_var_for_simult_subst"
+      ident(y) constr(A) constr(m) "as" ident(y') :=
+    let Hfresh := fresh in
+    let Heq := fresh in
+    let H1 := fresh in let H2 := fresh in let H3 := fresh in
+    pose proof (Hfresh := fresh_var_fresh y (quant_simult_subst_fvars y A m));
+    apply quant_simult_subst_fvars_inv in Hfresh as (H1&H2&H3);
+    remember (fresh_var y (quant_simult_subst_fvars y A m)) as y' eqn:Heq;
+    clear Heq.
+
+  Lemma simult_subst_id A m :
+    formula_fvars A ∩ dom m = ∅ →
+    simult_subst A m ≡ A.
+  Proof with auto.
+    induction A; simp simult_subst; intros.
+    - rewrite simult_subst_af_id...
+    - rewrite IHA...
+    - rewrite IHA1 by set_solver. rewrite IHA2 by set_solver...
+    - rewrite IHA1 by set_solver. rewrite IHA2 by set_solver...
+    - simpl. generalize_fresh_var_for_simult_subst x A m as y'.
+      intros σ. apply feval_exists_equiv_if. intros v. rewrite H...
+      + destruct H3.
+        * subst. rewrite fequiv_subst_diag...
+        * rewrite (fequiv_subst_trans A x y' (TConst v))...
+      + destruct H3.
+        * subst. rewrite fvars_subst_diag. set_solver.
+        * destruct (decide (x ∈ formula_fvars A)).
+          -- rewrite fvars_subst_free... set_solver.
+          -- rewrite fvars_subst_non_free... set_solver.
+  Qed.
+
+  Lemma simult_subst_term_empty t :
+    simult_subst_term t ∅ = t.
+  Proof. apply simult_subst_term_id. set_solver. Qed.
+
+  Lemma simult_subst_af_empty af :
+    simult_subst_af af ∅ = af.
+  Proof. apply simult_subst_af_id. set_solver. Qed.
+
+  Lemma simult_subst_empty A :
+    simult_subst A ∅ ≡ A.
+  Proof. apply simult_subst_id. set_solver. Qed.
+
+  Lemma simult_subst_term_delete_non_free t x m :
+    x ∉ term_fvars t →
+    simult_subst_term t m = simult_subst_term t (delete x m).
+  Proof with auto.
+    intros. induction t; simpl...
+    - simpl in H. apply not_elem_of_singleton in H. rewrite lookup_delete_ne...
+    - f_equal. induction args... simpl. f_equal.
+      + apply H0; [naive_solver | set_solver].
+      + apply IHargs.
+        * intros. apply H0... right...
+        * set_solver.
+  Qed.
+
+  Lemma simult_subst_af_delete_non_free af x m :
+    x ∉ af_fvars af →
+    simult_subst_af af m = simult_subst_af af (delete x m).
+  Proof with auto.
+    intros. destruct af; simpl...
+    - rewrite <- simult_subst_term_delete_non_free by set_solver.
+      rewrite <- simult_subst_term_delete_non_free by set_solver...
+    - f_equal. induction args... simpl. f_equal.
+      + rewrite <- simult_subst_term_delete_non_free... set_solver.
+      + apply IHargs. set_solver.
+  Qed.
+
+  Lemma simult_subst_delete_non_free A x m :
+    x ∉ formula_fvars A →
+    simult_subst A m ≡ simult_subst A (delete x m).
+  Proof with auto.
+    intros. induction A; simp simult_subst.
+    - rewrite <- simult_subst_af_delete_non_free...
+    - rewrite IHA...
+    - rewrite IHA1 by set_solver. rewrite IHA2 by set_solver...
+    - rewrite IHA1 by set_solver. rewrite IHA2 by set_solver...
+    - simpl. rename x0 into y.
+      generalize_fresh_var_for_simult_subst y A m as y1.
+      generalize_fresh_var_for_simult_subst y A (delete x m) as y2.
+      rewrite <- H0...
+      2: { admit. }
+      intros σ. apply feval_exists_equiv_if. intros v.
+      f_equiv. simpl.
+
+
+
+      (* rewrite <- H0... *)
+      (* +  *)
+
+
+  Lemma simult_subst_term_extract t0 x t m :
+    m !! x = Some t →
+    (term_fvars t ∩ dom (delete x m) = ∅) →
+    (x ∉ simult_subst_map_fvars (delete x m)) →
+    simult_subst_term t0 m = simult_subst_term (subst_term t0 x t) (delete x m).
+  Proof with auto.
+    induction t0; simpl; intros...
+    - destruct (decide (x0 = x)).
+      + subst. rewrite H. rewrite simult_subst_term_id...
+      + simpl. rewrite lookup_delete_ne...
+    - f_equal. induction args... simpl. f_equal.
+      + apply H... left...
+      + apply IHargs. intros. apply H... right...
+  Qed.
+
+  Lemma simult_subst_af_extract af x t m :
+    m !! x = Some t →
+    (term_fvars t ∩ dom (delete x m) = ∅) →
+    (x ∉ simult_subst_map_fvars (delete x m)) →
+    simult_subst_af af m = simult_subst_af (subst_af af x t) (delete x m).
+  Proof with auto.
+    destruct af; simpl; intros...
+    - simpl. f_equal; apply simult_subst_term_extract...
+    - simpl. f_equal. induction args... simpl. f_equal...
+      apply simult_subst_term_extract...
+  Qed.
+
+  Lemma simult_subst_extract A x t m :
+    m !! x = Some t →
+    (term_fvars t ∩ dom (delete x m) = ∅) →
+    (x ∉ simult_subst_map_fvars (delete x m)) →
+    simult_subst A m ≡ simult_subst (A[x \ t]) (delete x m).
+  Proof with auto.
+    induction A; simp simult_subst; simpl; intros.
+    - rewrite simpl_subst_af. rewrite (simult_subst_af_extract af x t m)...
+    - rewrite simpl_subst_not. simp simult_subst. rewrite IHA...
+    - rewrite simpl_subst_and. simpl. simp simult_subst. rewrite IHA1... rewrite IHA2...
+    - rewrite simpl_subst_or. simpl. simp simult_subst. rewrite IHA1... rewrite IHA2...
+    - rename x0 into y. destruct (decide (x = y)).
+      + subst. rewrite simpl_subst_exists_skip... simp simult_subst.
+        simpl.
+        generalize_fresh_var_for_simult_subst y A m as y1.
+        generalize_fresh_var_for_simult_subst y A (delete y m) as y2.
+        admit.
+      + rewrite simpl_subst_exists_propagate.
+        2: { admit. }
+        2: { admit. }
+        generalize_fresh_var_for_simult_subst y A m as y1.
+        generalize_fresh_var y A x t as y2.
+        simp simult_subst.
+        constr ident constr as ident
+        generalize_fresh_var_for_simult_subst y A (delete y m) as y2.
+        rewrite simult_subst_non_free.
+
+      +
+      destruct (decide ())
+
+
+
+      generalize_fresh_var_for_simult_subst x A (∅ : gmap variable term) as y'.
+      intros σ. apply feval_exists_equiv_if. intros v. rewrite H...
+      destruct H2.
+      + subst. rewrite fequiv_subst_diag...
+      + rewrite (fequiv_subst_trans A x y' (TConst v))...
+  Qed.
+End simult_subst.
